providers/evercrypt/EverCrypt.Hash.fsti
@@ -23,35 +23,47 @@ let state alg = B.pointer (state_s alg)
 
 // NS: note that the state is the first argument to the invariant so that we can
 // do partial applications in pre- and post-conditions
-val invariant_s: (#a: e_alg) -> state_s a -> HS.mem -> Type0
-let invariant (#a: e_alg) (s: state a) (m: HS.mem) =
-  B.live m s /\ invariant_s (B.get m s 0) m
 val footprint_s: #a:e_alg -> state_s a -> GTot M.loc
 let footprint (#a: e_alg) (s: state a) (m: HS.mem) =
-  M.(loc_union (loc_buffer s) (footprint_s (B.get m s 0)))
+  M.(loc_union (loc_buffer s) (footprint_s (deref m s)))
+
+val invariant_s: (#a: e_alg) -> state_s a -> HS.mem -> Type0
+let invariant (#a: e_alg) (s: state a) (m: HS.mem) =
+  B.live m s /\
+  M.(loc_disjoint (loc_buffer s) (footprint_s (deref m s))) /\
+  invariant_s (B.get m s 0) m
 
 let type_of alg =
   match G.reveal alg with
   | SHA256 -> uint_32
   | SHA384 -> uint_64
 
-let size_of alg =
+let size_of_k alg =
   match G.reveal alg with
-  | SHA256 -> 8
-  | SHA384 -> 8
+  | SHA256 -> 64
+  | SHA384 -> 80
 
-let repr_t (a: e_alg) =
-  Seq.lseq (type_of a) (size_of a)
+type repr_t (a: e_alg) = {
+  k: Seq.lseq (type_of a) (size_of_k a);
+  hash: Seq.lseq (type_of a) 8;
+  counter: nat;
+}
 
 val repr: #a:e_alg -> s:state a -> h:HS.mem { invariant s h } ->
   GTot (repr_t a)
 
+// Waiting for these to land in LowStar.Modifies
+let loc_in (l: M.loc) (h: HS.mem) =
+  M.(loc_not_unused_in h `loc_includes` l)
 
-// TODO: define these over memory locations
-val used_in: M.loc -> HS.mem -> Type0
-val fresh_loc: M.loc -> HS.mem -> HS.mem -> Type0
+let loc_unused_in (l: M.loc) (h: HS.mem) =
+  M.(loc_unused_in h `loc_includes` l)
+
+let fresh_loc (l: M.loc) (h0 h1: HS.mem) =
+  loc_unused_in l h0 /\ loc_in l h1
+
 val fresh_is_disjoint: l1:M.loc -> l2:M.loc -> h0:HS.mem -> h1:HS.mem -> Lemma
-  (requires (fresh_loc l1 h0 h1 /\ l2 `used_in` h0))
+  (requires (fresh_loc l1 h0 h1 /\ l2 `loc_in` h0))
   (ensures (M.loc_disjoint l1 l2))
 
 val frame_invariant: #a:e_alg -> l:M.loc -> s:state a -> h0:HS.mem -> h1:HS.mem -> Lemma
@@ -86,8 +98,16 @@ val create: a:alg -> ST (state (G.hide a))
 
 let init_repr (a: e_alg): GTot (repr_t a) =
   match G.reveal a with
-  | SHA256 -> EverCrypt.Spec.SHA2_256.h_0
-  | SHA384 -> EverCrypt.Spec.SHA2_384.h_0
+  | SHA256 -> {
+      hash = EverCrypt.Spec.SHA2_256.h_0;
+      k = EverCrypt.Spec.SHA2_256.k;
+      counter = 0
+    }
+  | SHA384 -> {
+      hash = EverCrypt.Spec.SHA2_384.h_0;
+      k = EverCrypt.Spec.SHA2_384.k;
+      counter = 0
+    }
 
 val init: #a:e_alg -> s:state a -> ST unit
   (requires (invariant s))
