providers/evercrypt/EverCrypt.ValeGlue.fsti
@@ -2,15 +2,35 @@
 module EverCrypt.ValeGlue
 
 open EverCrypt.Helpers
+open FStar.HyperStack.ST
+
+module U32 = FStar.UInt32
+module B = LowStar.Buffer
+module M = LowStar.Modifies
+module HS = FStar.HyperStack
+
+type uint8_p = B.buffer UInt8.t
 
 ///  SHA256
 
+// JP: no clue that this is correct ...
+let sha256_size_state = 137ul
+
+type sha256_state = b:B.buffer UInt32.t { B.length b = U32.v sha256_size_state }
+
+val sha256_slice_k: HS.mem -> sha256_state -> Seq.lseq UInt32.t 64
+val sha256_slice_hash: HS.mem -> sha256_state -> Seq.lseq UInt32.t 8
+val sha256_counter: HS.mem -> sha256_state -> nat
+
 /// Incremental API
-val sha256_init: state:uint32_p -> Stack_ unit
-val sha256_update: state:uint32_p -> data:uint8_p -> Stack_ unit
-val sha256_update_multi: state:uint32_p -> data:uint8_p -> n:uint32_t -> Stack_ unit
-val sha256_update_last: state:uint32_p -> data:uint8_p -> n:uint32_t -> Stack_ unit
-val sha256_finish: state:uint32_p -> data:uint8_p -> Stack_ unit
+val sha256_init: state:B.buffer UInt32.t ->
+  Stack unit
+    (requires (fun h0 -> B.live h0 state))
+    (ensures (fun h0 _ h1 -> B.live h1 state /\ M.(modifies (loc_buffer state) h0 h1)))
+val sha256_update: state:sha256_state -> data:uint8_p -> Stack_ unit
+val sha256_update_multi: state:sha256_state -> data:uint8_p -> n:uint32_t -> Stack_ unit
+val sha256_update_last: state:sha256_state -> data:uint8_p -> n:uint32_t -> Stack_ unit
+val sha256_finish: state:sha256_state -> data:uint8_p -> Stack_ unit
 
 /// All-in one
 val sha256_hash: dst:uint8_p -> data:uint8_p -> n:uint32_t -> Stack_ unit
