providers/evercrypt/fst/EverCrypt.Hash.fst
@@ -3,27 +3,33 @@ module EverCrypt.Hash
 open EverCrypt.Helpers
 open FStar.HyperStack.ST
 
+module U32  = FStar.UInt32
 module HS = FStar.HyperStack
 module B = LowStar.Buffer
 module M = LowStar.Modifies
 module G = FStar.Ghost
+module T = LowStar.ToFStarBuffer
+
+module AC = EverCrypt.AutoConfig
+module SC = EverCrypt.StaticConfig
+module Vale = EverCrypt.Vale
+module Hacl = EverCrypt.Hacl
+module ValeGlue = EverCrypt.ValeGlue
+
+module ST = FStar.HyperStack.ST
+module MP = LowStar.ModifiesPat
 
 open LowStar.BufferOps
 open FStar.Integers
-
-#reset-options "--using_facts_from '* -Hacl -Spec'"
 
 let uint32_p = B.buffer uint_32
 let uint64_p = B.buffer uint_64
 
 noeq
 type state_s: (G.erased alg) -> Type0 =
-| SHA256_Hacl: p:uint32_p{ B.length p = 8 } -> state_s (G.hide SHA256)
-| SHA256_Vale: p:uint32_p{ B.length p = 8 } -> state_s (G.hide SHA256)
-| SHA384_Hacl: p:uint64_p{ B.length p = 8 } -> state_s (G.hide SHA384)
-
-let invariant_s #_ _ _ =
-  True
+| SHA256_Hacl: p:uint32_p{ B.length p = U32.v Hacl.SHA2_256.size_state } -> state_s (G.hide SHA256)
+| SHA256_Vale: p:uint32_p{ B.length p = U32.v ValeGlue.sha256_size_state } -> state_s (G.hide SHA256)
+| SHA384_Hacl: p:uint64_p{ B.length p = U32.v Hacl.SHA2_384.size_state } -> state_s (G.hide SHA384)
 
 let footprint_s #a (s: state_s a): GTot M.loc =
   match s with
@@ -31,12 +37,86 @@ let footprint_s #a (s: state_s a): GTot M.loc =
   | SHA256_Vale p -> M.loc_buffer p
   | SHA384_Hacl p -> M.loc_buffer p
 
+let invariant_s #a s h =
+  match s with
+  | SHA256_Hacl p ->
+      B.live h p
+  | SHA256_Vale p ->
+      B.live h p
+  | SHA384_Hacl p ->
+      B.live h p
+
 let repr #a s h: GTot _ =
   let s = B.get h s 0 in
   match s with
   | SHA256_Hacl p ->
-      B.as_seq h p
+      let p = T.new_to_old_ghost p in
+      {
+        k = Hacl.SHA2_256.slice_k h p;
+        hash = Hacl.SHA2_256.slice_hash h p;
+        counter = Hacl.SHA2_256.counter h p
+      }
   | SHA256_Vale p ->
-      B.as_seq h p
+      {
+        k = ValeGlue.sha256_slice_k h p;
+        hash = ValeGlue.sha256_slice_hash h p;
+        counter = ValeGlue.sha256_counter h p
+      }
   | SHA384_Hacl p ->
-      B.as_seq h p
+      {
+        k = Seq.create 80 0UL;
+        hash = Seq.create 8 0UL;
+        counter = 0
+      }
+
+let repr_eq (#a:e_alg) (r1 r2: repr_t a) =
+  Seq.equal r1.k r2.k /\
+  Seq.equal r1.hash r2.hash /\
+  r1.counter = r2.counter
+
+let fresh_is_disjoint l1 l2 h0 h1 =
+  ()
+
+let frame_invariant #a l s h0 h1 =
+  let state = deref h0 s in
+  // Note: the Vale functions are still uninterpreted, meaning that we can't
+  // derive that they output is preserved as long as the state is not modified.
+  assume (not (SHA256_Vale? state));
+  assert (repr_eq (repr s h0) (repr s h1))
+
+let create a =
+  let h0 = ST.get () in
+  let i = AC.sha256_impl () in
+  let s: state_s (G.hide a) =
+    match a with
+    | SHA256 ->
+        if SC.vale && i = AC.Vale then
+          let b = B.malloc HS.root 0ul Hacl.SHA2_256.size_state in
+          SHA256_Vale b
+        else
+          let b = B.malloc HS.root 0ul ValeGlue.sha256_size_state in
+          SHA256_Hacl b
+    | SHA384 ->
+        let b = B.malloc HS.root 0UL Hacl.SHA2_384.size_state in
+        SHA384_Hacl b
+  in
+  let h1 = ST.get () in
+  let r = B.malloc HS.root s 1ul in
+  let h2 = ST.get () in
+  // None of these seem to be necessary for the proof to proceed. Key bits are
+  // retained.
+  assert (invariant r h2);
+  assert (fresh_loc (M.loc_buffer r) h1 h2);
+  assert (M.(modifies loc_none h0 h1));
+  assert (loc_unused_in (M.loc_buffer r) h0);
+  assert (M.(modifies loc_none h0 h2));
+  r
+
+#set-options "--z3rlimit 20"
+
+let init #a s =
+  match !*s with
+  | SHA256_Hacl p ->
+      Hacl.SHA2_256.init (T.new_to_old_st p)
+  | _ ->
+      admit ()
