providers/evercrypt/EverCrypt.AutoConfig.fsti
@@ -3,6 +3,8 @@ module EverCrypt.AutoConfig
 open EverCrypt.Helpers
 open FStar.HyperStack.ST
 
+module M = LowStar.Modifies
+
 /// Multiplexing support
 type impl = | Hacl | Vale | OpenSSL | BCrypt
 
@@ -10,7 +12,9 @@ type cfg =
 | Default
 | Prefer: preferred:impl -> cfg
 
-let getter a = unit -> Stack_ a
+let getter a = unit -> Stack a
+  (requires (fun _ -> true))
+  (ensures (fun h0 _ h1 -> M.(modifies loc_none h0 h1)))
 val sha256_impl: getter impl
 val sha384_impl: getter impl
 val sha512_impl: getter impl
